\input{default}

\begin{document}
	$$I = \int \limits_{0}^{\frac{\pi}{2}} \frac{\tan^{-1} (\sin t)}{\sin t} dt = \sum_{n = 0}^{\infty} \frac{(-1)^n}{2n+1} \int \limits_{0}^{\frac{\pi}{2}} (\sin t)^{2n} \; dt=$$
	$$= \sum_{n = 0}^{\infty} \frac{(-1)^n}{2n+1} \cdot \frac{(2n-1)!!}{(2n)!!} \cdot \frac{\pi}{2} $$
	$$ \frac{1}{2n+1} = \frac{1}{2} \cdot \frac{1}{n+\frac{1}{2}} = \frac{1}{2} \cdot \frac{(1/2)_n}{\frac{1}{2} (3/2)_n} = \frac{(1/2)_n}{(3/2)_n} $$
	$$\frac{(2n-1)!!}{(2n)!!} = \frac{(n-\frac{1}{2})\cdot ... \cdot \frac{1}{2}}{n \cdot ... \cdot 1} = \frac{(1/2)_n}{(1)_n}$$
	$$I = \frac{\pi}{2} \sum_{n = 0}^{\infty} \frac{(1/2)_n (1/2)_n}{(3/2)_n (1)_n} (-1)^n = \frac{\pi}{2} {}_2F_1 \Big(\begin{array}{c}
		\frac{1}{2}, \frac{1}{2} \\ \frac{3}{2}
	\end{array}; -1\Big)$$
	$${}_2F_1 \Big(\begin{array}{c}
		a, b \\ c
	\end{array}; z\Big) = \frac{\Gamma(c)}{\Gamma(b) \Gamma(c-b) } \int \limits_0^1 t^{b-1} (1-t)^{c-b-1} (1-tz)^{-a} \; dt$$
	$$a = b = \frac{1}{2}; \quad c = \frac{3}{2}; \quad z = -1$$
	$${}_2F_1 \Big(\begin{array}{c}
		\frac{1}{2}, \frac{1}{2} \\ \frac{3}{2}
	\end{array}; -1\Big) = \frac{\Gamma(3/2)}{\Gamma(1/2) \Gamma(1) } \int \limits_0^1 t^{-1/2} (1-t)^{0} (1+t)^{-1/2} \; dt = $$
	$$= \frac{1}{2} \int \limits_0^1 \frac{dt}{\sqrt{t^2+t}} = \frac{1}{2} \int \limits_0^1 \frac{dt}{\sqrt{(t+\frac{1}{2})^2-(\frac{1}{2})^2}} =$$
	$$= \left[\begin{array}{c}
		t+\frac{1}{2} = \frac{1}{2} \cosh \theta \\ dt =  \frac{1}{2} \sinh \theta \; d\theta 
	\end{array}\right] = \frac{1}{2}\int \limits_0^{\cosh^{-1} 3} \frac{\frac{1}{2} \sinh \theta \; d\theta}{\frac{1}{2} \sinh \theta} = \frac{1}{2}  \cosh^{-1} 3 = \ln(1+\sqrt{2})$$
	$$I = \frac{\pi}{2} \ln (1+\sqrt{2})$$
\end{document}