\input{default}

\begin{document}
	$$I = \int \limits_0^{\infty} \frac{(\ln x)^2 \arcctg x}{x^2+1} \; dx = \left[\begin{array}{c}
		x = 1/t\\ dx = -dt/t^2 
	\end{array}\right] =$$
	$$=\int \limits_{\infty}^0 \frac{(\ln t)^2 (\frac{\pi}{2}-\arcctg t)}{\frac{1}{t^2}+1} \cdot \Big(-\frac{1}{t^2}\Big) \; dt = \frac{\pi}{2} \int \limits_0^{\infty} \frac{(\ln t)^2 }{t^2+1} \; dt - I$$
	$$I =\frac{\pi}{4} \int \limits_0^{\infty} \frac{(\ln t)^2 }{t^2+1} \; dt $$ 
	$$J(a) = \int \limits_0^{\infty} \frac{t^a }{t^2+1} \; dt $$
	$$I = \frac{\pi}{4} J''(0)$$
	$$J(a) = \int \limits_0^{\infty} \frac{t^a }{t^2+1} \; dt = \left[\begin{array}{c}
		t = \tan \theta \\ dt  = \sec^2 \theta d\theta 
	\end{array}\right] =\int \limits_0^{\frac{\pi}{2}} \tan^a \theta \; d\theta = $$
	$$\frac{1}{2} \cdot 2 \int \limits_0^{\frac{\pi}{2}} \sin^{2\frac{a+1}{2}-1} \theta \cos^{2\frac{1-a}{2}-1} \theta \; d\theta = \frac{1}{2} B\Big(\frac{a+1}{2}; \frac{1-a}{2}\Big)=$$
	$$= \frac{1}{2} \frac{\Gamma(\frac{a+1}{2}) \Gamma(\frac{a+1}{2})}{\Gamma(1)} = \frac{1}{2} \Gamma\Big(\frac{a+1}{2}\Big) \Gamma\Big(\frac{a+1}{2}\Big)=$$
	$$= \frac{\pi}{2 \sin (\pi \cdot \frac{a+1}{2})} = \frac{\pi}{2} \cdot \frac{1}{\sin (\frac{\pi}{2} (a+1))} $$
	$$J' = \frac{\pi}{2} \cdot \frac{-\frac{\pi}{2} \cdot \cos (\frac{\pi}{2} (a+1))}{\sin^2(\frac{\pi}{2} (a+1))} = -\frac{\pi^2}{4} \cdot \frac{\cos (\frac{\pi}{2} (a+1))}{\sin^2(\frac{\pi}{2} (a+1))}$$
	$$J'' = -\frac{\pi^2}{4} \cdot \frac{-\frac{\pi}{2} \cdot \sin^3 (\frac{\pi}{2} (a+1))-\cos(\frac{\pi}{2} (a+1)) \cdot \partial_a \sin^2 (\frac{\pi}{2} (a+1)) }{\sin^4 (\frac{\pi}{2} (a+1))}$$
	$$J''(0) = \frac{\pi^3}{8}$$
	$$I = \frac{\pi}{4} \cdot \frac{\pi^3}{8} = \frac{\pi^4}{32}$$
\end{document}