\input{default.tex}

\begin{document}
	$$\prod_{n = 1}^{\infty} \bigg(\frac{n! e^n}{\sqrt{2\pi n} n^n}\bigg)^{(-1)^{n-1}} = P$$
	$$\ln P = \sum_{n = 1}^{\infty} (-1)^{n-1} \ln n! - \sum_{n = 1}^{\infty} (-1)^{n-1} \ln \sqrt{2\pi n} \bigg(\frac{n}{e}\bigg)^n$$
	$$\sum_{n = 1}^{\infty} (-1)^{n-1} \ln n! = \sum_{n = 1}^{\infty} (-1)^{n-1} \sum_{k = 1}^{n} \ln k = \sum_{n = 1}^{\infty} \sum_{k = 1}^{n}  (-1)^{n-1} \ln k =$$
	$$= \sum_{k = 1}^{\infty} \sum_{n = k}^{\infty}  (-1)^{n-1} \ln k = \sum_{k = 1}^{\infty} \ln k \sum_{n = k}^{\infty} (-1)^{n-1} = \frac{1}{2} \sum_{k = 1}^{\infty} (-1)^{k-1} \ln k$$
	$$\sum_{n = 1}^{\infty} (-1)^{n-1} \ln \sqrt{2\pi n} \bigg(\frac{n}{e}\bigg)^n = \sum_{n = 1}^{\infty} (-1)^{n-1} \bigg{[} \frac{1}{2} \ln 2\pi +\frac{1}{2} \ln n +n\ln n - n \bigg{]}=$$
	$$= \frac{1}{2} \eta(0) \ln 2\pi  + \frac{1}{2} \sum_{k = 1}^{\infty} (-1)^{k-1} \ln k + \sum_{n = 1}^{\infty} (-1)^{n-1} n \ln n - \eta(-1)=$$
	$$= \frac{1}{4} \ln 2\pi - \frac{1}{4} +  \frac{1}{2} \sum_{k = 1}^{\infty} (-1)^{k-1} \ln k + \sum_{n = 1}^{\infty} (-1)^{n-1} n \ln n$$
	$$\ln P = \frac{1}{2} \sum_{k = 1}^{\infty} (-1)^{k-1} \ln k - \frac{1}{4} \ln 2\pi + \frac{1}{4} -  \frac{1}{2} \sum_{k = 1}^{\infty} (-1)^{k-1} \ln k - \sum_{n = 1}^{\infty} (-1)^{n-1} n \ln n =$$
	$$= - \frac{1}{4} \ln 2\pi + \frac{1}{4} - \sum_{n = 1}^{\infty} (-1)^{n-1} n \ln n$$
	$$\sum_{n = 1}^{\infty} (-1)^{n-1} n \ln n = \frac{d}{dx} \bigg{|}_{x = 1} \sum_{n = 1}^{\infty} (-1)^{n-1} n^x = \frac{d}{dx} \bigg{|}_{x = 1} \eta(-x) =$$
	$$= \frac{d}{dx} \bigg{|}_{x = 1} (1-2^{1+x})\zeta(-x) = (1-2^{1+x})\zeta(-x) \bigg{[} \frac{-2^{1+x}\ln 2}{1-2^{1+x}} - \frac{\zeta'(-x)}{\zeta(-x)} \bigg{]} \bigg{|}_{x = 1} =$$
	$$=-4\zeta(-1) \ln 2 - (1 - 4)\zeta'(-1) = \frac{1}{3}\ln 2 + 3 (\frac{1}{12} - \ln A) = \frac{1}{4} + \frac{1}{3} \ln 2 -  3\ln A$$
	$$\ln P = - \frac{1}{4} \ln 2\pi + \frac{1}{4} - \frac{1}{4} - \frac{1}{3} \ln 2 +  3\ln A = -\frac{7}{12} \ln 2 - \frac{1}{4} \ln \pi + 3\ln A$$
	$$P = \frac{A^3}{2^{7/12} \pi^{1/4}}$$
\end{document}