\input{default}

\begin{document}
	$$S = 1+\sum_{n= 1}^{\infty} \frac{(2n-1)!!}{(2n)!!} \cdot \frac{1}{(4n+1)^2}$$
	$$4n+1 = 4\Big(n+\frac{1}{4}\Big) = \frac{(5/4)_n}{(1/4)_n}$$
	$$S = 1+\sum_{n= 1}^{\infty} \frac{(1/2)_n (1/4)_n^2}{(1)_n (5/4)_n} = {}_3F_2 \Big(\begin{array}{c}
		\frac{1}{2}, \frac{1}{4},\frac{1}{4}  \\ \frac{5}{4}, \frac{5}{4}
	\end{array}; 1\Big)$$
	$${}_3F_2 \Big(\begin{array}{c}
		a, b, c  \\ 1+a-b, 1+a-c
	\end{array}; 1\Big) = \frac{\Gamma(1+\frac{a}{2}) \Gamma(1+a-b) \Gamma(1+a-c) \Gamma(1+\frac{a}{2}-b-c)}{\Gamma(1+a) \Gamma(1+\frac{a}{2}-b) \Gamma(1+\frac{a}{2}-c) \Gamma(1+a-b-c)}$$
	$$a = \frac{1}{2}, \quad  b = \frac{1}{4}, \quad c = \frac{1}{4}$$
	$$S = \frac{\Gamma(\frac{5}{4}) \Gamma(\frac{5}{4}) \Gamma(\frac{5}{4}) \Gamma(\frac{3}{4})}{\Gamma(\frac{3}{2}) } = \frac{2}{4^3} \frac{ \Gamma^2(\frac{1}{4})\sqrt{2} \pi}{\sqrt{\pi}} = \frac{\sqrt{2\pi}}{32} \Gamma^2\Big(\frac{1}{4}\Big)$$
	
	
\end{document}