\input{default}

\begin{document}
	$$S = 5 \Big( \frac{1}{2}\Big)^3 \Big( 1+ \frac{1}{2} \Big)-9 \Big(\frac{1\cdot 3}{2 \cdot 4}\Big)^3 \Big( 1+ \frac{1}{2}+\frac{1}{3}+\frac{1}{4} \Big)+ ... =\sum_{n= 1}^{\infty} (4n+1)\left[ \frac{(2n-1)!!}{(2n)!!} \right]^3 H_{2n} (-1)^{n-1}$$
	$$4n+1 = \frac{(5/4)_n}{(1/4)_n}$$
	$$H_{2n} = \frac{1}{2} \frac{(1)_n}{(1/2)_n}\partial_c \Big|_{c = \frac{1}{2}} \frac{(c)_n}{(\frac{3}{2} - c)_n}$$
	$$S = - \frac{1}{2} \partial_c \Big|_{c = \frac{1}{2}} \sum_{n= 1}^{\infty} \frac{(5/4)_n}{(1/4)_n}\left[ \frac{(1/2)_n}{(1)_n} \right]^3 \frac{(1)_n (c)_n}{(1/2)_n (\frac{3}{2} - c)_n} (-1)^n$$
	$$S = - \frac{1}{2}  \partial_c \Big|_{c = \frac{1}{2}} {}_4F_3 \Big(\begin{array}{c}
		\frac{5}{4}, \frac{1}{2}, \frac{1}{2}, c  \\ \frac{1}{4}, 1, \frac{3}{2}-c
	\end{array}; -1\Big) $$
	$${}_4F_3 \Big(\begin{array}{c}
		a, 1+\frac{a}{2}, b, c  \\ \frac{a}{2}, a-b+1, a-c+1
	\end{array}; -1\Big) = \frac{\Gamma(a-b+1) \Gamma(a-c+1)}{\Gamma(1+a) \Gamma(a-b-c+1) }$$
	$$a = b = \frac{1}{2}$$
	$$S =-\frac{1}{2} {}_4F_3 \Big(\begin{array}{c}
		\frac{5}{4}, \frac{1}{2}, \frac{1}{2}, \frac{1}{2} \\ \frac{1}{4}, 1, 1
	\end{array}; -1\Big) \Big( -\psi(1)+\psi(1/2)\Big) =  \frac{2}{\pi}  \ln2 $$
	
	
	
\end{document}