\input{default}

\begin{document}
	$$S = \sum_{n = 0}^{\infty} \frac{ (n!)^2}{(2n)!} = 1 + \sum_{n = 1}^{\infty} \frac{n \Gamma(n) \Gamma(n+1)}{\Gamma(2n+1)} =1 + \sum_{n = 1}^{\infty} n B(n, n+1)$$
	$$S-1=   \sum_{n = 1}^{\infty} n \int \limits_0^1 t^{n} (1-t)^{n-1}\; dt = \int \limits_0^1 t \sum_{n = 1}^{\infty} n (t(1-t))^{n-1}\; dt =  \left[ \begin{array}{c} z = t(1-t) \\ |z|< 1 \end{array} \right] =$$
	$$=    \int \limits_0^1 t \frac{d}{dz}\sum_{n = 1}^{\infty} z^n\; dt =  \int \limits_0^1 t \frac{d}{dz}\sum_{n = 0}^{\infty} z^n\; dt = \int \limits_0^1 t \frac{d}{dz} \Bigg( \frac{1}{1-z}\Bigg) \; dt=$$
	$$= \int \limits_0^1 \frac{t}{(1-z)^2}  \; dt= \int \limits_0^1 \frac{t}{(1-t(1-t))^2}  \; dt =  \int \limits_0^1 \frac{t}{(t^2-t+1)^2}  \; dt =$$
	$$= \int \limits_0^1 \frac{t-\frac{1}{2}+\frac{1}{2}}{((t-\frac{1}{2})^2+\frac{3}{4})^2}  \; dt = \int \limits_{-\frac{1}{2}}^{\frac{1}{2}} \frac{u+\frac{1}{2}}{(u^2+\frac{3}{4})^2}  \; du = \frac{1}{2} \int \limits_{-\frac{1}{2}}^{\frac{1}{2}} \frac{du}{(u^2+\frac{3}{4})^2} = $$
	$$= \left[ \begin{array}{c} u = \frac{\sqrt{3}}{2} \tan \theta \\ du = \frac{\sqrt{3}}{2} \sec^2 \theta \; d\theta \end{array} \right] = \frac{1}{2} \int \limits_{-\frac{\pi}{6}}^{\frac{\pi}{6}} \frac{\frac{\sqrt{3}}{2} \sec^2 \theta \; d\theta}{\frac{9}{16} \sec^4 \theta} = \frac{4\sqrt{3}}{9} \int \limits_{-\frac{\pi}{6}}^{\frac{\pi}{6}} \cos^2 \theta \; d\theta =$$
	$$= \frac{4\sqrt{3}}{9} \int \limits_{-\frac{\pi}{6}}^{\frac{\pi}{6}} \frac{1+\cos 2\theta}{2} \; d\theta = \frac{2\sqrt{3}}{9} \cdot \frac{\pi}{3} + \frac{\sqrt{3}}{9} \cdot 2 \cdot \frac{\sqrt{3}}{2} = \frac{2\pi\sqrt{3}}{27}+\frac{1}{3}$$
	$$S = \frac{2\pi\sqrt{3}}{27}+\frac{4}{3}$$
	
\end{document}