\input{default}

\begin{document}
	$$S = \sum_{n = 0}^{\infty} \sum_{m = 0}^{\infty} \frac{m+n+mn}{2^m (2^m+2^n)} = \frac{1}{2}\Bigg(\sum_{n = 0}^{\infty} \sum_{m = 0}^{\infty} \frac{m+n+mn}{2^m (2^m+2^n)}+\sum_{n = 0}^{\infty} \sum_{m = 0}^{\infty} \frac{m+n+mn}{2^n (2^m+2^n)}\Bigg) =$$
	$$=\frac{1}{2}\Bigg(\sum_{n = 0}^{\infty} \sum_{m = 0}^{\infty} \frac{m+n+mn}{2^m+2^n} (\frac{1}{2^n}+\frac{1}{2^m}\Bigg) = \frac{1}{2}\Bigg(\sum_{n = 0}^{\infty} \sum_{m = 0}^{\infty} \frac{m+n+mn}{2^{m+n}}\Bigg)=$$
	$$= \frac{1}{2}\Bigg(\sum_{n = 0}^{\infty} \frac{1}{2^n} \sum_{m = 0}^{\infty} \frac{m}{2^m} + \sum_{n = 0}^{\infty} \frac{n}{2^n} \sum_{m = 0}^{\infty} \frac{1}{2^m} + \sum_{n = 0}^{\infty} \frac{n}{2^n} \sum_{m = 0}^{\infty} \frac{m}{2^m}\Bigg)$$
	$$\sum_{n = 0}^{\infty} \frac{1}{2^n} = 2$$
	$$\sum_{n = 0}^{\infty} \frac{n}{2^n} = \sum_{n = 0}^{\infty} n \Delta(-2\cdot 2^{-n}) = n\cdot (-2\cdot 2^{-n}) \Bigg|_{0}^{\infty}-\sum_{n = 1}^{\infty} (-2\cdot 2^{-n}) \Delta n = $$
	$$= 2\sum_{n = 1}^{\infty} ( 2^{-n}) = 2$$
	$$S = \frac{1}{2} (2\cdot 2+2\cdot 2+2\cdot 2) = 6$$
	
\end{document}