\input{default}

\begin{document}
	$$S = \sum_{n = 1}^{\infty} \frac{1}{2^n (1+2^{2^{-n}})} = \left[\begin{array}{c} u =2^{2^{-n}} \\ \frac{1}{1+u} = \frac{2}{1-u^2} - \frac{1}{1-u} 
	\end{array}\right] =$$
	$$= \frac{1}{2(1+\sqrt{2})} + \sum_{n = 2}^{\infty} \frac{2}{2^n (1+(2^{2^{-n}})^2)} - \frac{1}{2^n (1+2^{2^{-n}})} = $$
	$$= \frac{1}{2(1+\sqrt{2})} + \sum_{n = 2}^{\infty} \frac{1}{2^{n-1} (1+2^{2^{-(n-1)}})} - \frac{1}{2^n (1+2^{2^{-n}})}$$
	$$f(n) = \frac{1}{2^n (1+2^{2^{-n}})}$$
	$$S= \frac{1}{2(1+\sqrt{2})} + f(1) - \lim_{n \to \infty} f(n)=$$
	$$=  \frac{1}{2(1+\sqrt{2})} + \frac{1}{2(1-\sqrt{2})}- \lim_{n \to \infty} \frac{2^{-n}}{ 1+2^{2^{-n}}} = -1-L$$
	$$L = \lim_{n \to \infty} \frac{2^{-n}}{ 1+2^{2^{-n}}} = \lim_{n \to \infty} \frac{-\ln2 \cdot 2^{-n}}{ \ln^2 2 \cdot 2^{-n} \cdot 2^{2^{-n}}} = -\frac{1}{\ln 2}$$
	$$S = \frac{1}{\ln 2} - 1$$
	
\end{document}