\input{default}

\begin{document}
	$$S = \sum_{n= 2}^{\infty} \frac{n^4+n^3+n^2-n+1}{n^6-1} $$
	$$ \frac{n^4+n^3+n^2-n+1}{n^6-1} = \frac{1/2}{n-1}+\frac{-1/2}{n+1}+\frac{A+A'n}{n^2-n+1}+\frac{B+B'n}{n^2+n+1}=$$
	$$= \frac{1}{n^2-1}+\frac{A+A'n}{n^2-n+1}+\frac{B+B'n}{n^2+n+1}$$
	$$n^4+n^3+n^2-n+1 = (n^2-n+1)(n^2+n+1)+(A+A'n)(n^2-1)(n^2+n+1)+$$
	$$+(B+B'n)(n^2-1)(n^2-n+1)$$
	Приравняем коэффициенты при степенях n:
	\newline
	$5: \; A'+B' = 0$
	\newline
	$4: \; A+B+1 = 1$
	\newline
	$3: \; A-B = 1$
	\newline
	$2: \; 1-A'+B' = 1$
	\newline
	$1: \; -A+B-A'-B' = -1$
	\newline
	$0: \; 1-A-B = 1$
	\newline
	$$\begin{cases}
		A'=B' = 0\\
		A = \dfrac{1}{2}\\
		B =  -\dfrac{1}{2}
	\end{cases}$$
	$$S = \frac{1}{2} \sum_{n= 2}^{\infty} \Bigg(\frac{1}{n-1}-\frac{1}{n+1}\Bigg)+\frac{1}{2} \sum_{n= 2}^{\infty} \Bigg(\frac{1}{n^2-n+1}-\frac{1}{n^2+n+1}\Bigg)=$$
	$$= \frac{1}{2} \sum_{n= 2}^{\infty} \Bigg(\frac{1}{n-1}-\frac{1}{n+1}\Bigg)+\frac{1}{2} \sum_{n= 2}^{\infty} \Bigg(\frac{1}{(n-\frac{1}{2})^2+\frac{3}{4}}-\frac{1}{(n+\frac{1}{2})^2+\frac{3}{4}}\Bigg)=$$
	$$=\frac{1}{2} \Bigg( \Big(1+\frac{1}{2}\Big)+ \frac{1}{\frac{9}{4}+\frac{3}{4}}  \Bigg) = \frac{1}{2}\Bigg( \frac{3}{2} +\frac{1}{3} \Bigg) = \frac{11}{12}$$
	
\end{document}